Clean/Gadgets/Keccak/ThetaC.lean
@@ -23,6 +23,8 @@ def Spec (state : KeccakState (F p)) (out : KeccakRow (F p)) :=
   out.Normalized
   ∧ out.value = Specs.Keccak256.thetaC state.value
 
+set_option debug.explicitCircuitReduced true
+
 -- #eval! theta_c (p:=p_babybear) default |>.localLength
 set_option maxHeartbeats 20000 in
 @[reducible]
